theories/FOL/Undecidability/FSAT_direct_undec.v
@@ -96,11 +96,37 @@ Section Fragment.
         apply DecidabilityFacts.decidable_iff'; destruct I.
         1: now exists fP. 1: now exists fL. now exists fE.
   Qed.
-(* TODO 
-  Theorem FSATdc_undec :
+
+  Theorem FSATdc_undec_frag :
     undecidable FSATdc.
   Proof.
-   apply (undecidability_from_reducibility FSATd_undec).
-   apply FSATd_to_FSATdc.reduction.
-  Qed. *)
+    apply (undecidability_from_reducibility FSATdc_undec).
+    unshelve eexists translate_form_closed. 1-2: unfold Dec.dec; repeat decide equality.
+    intros [k Hclosed]. split; intros (D & I & rho & (l & Hlist) & Hdisc & Hdec & H).
+    - exists D, (full_tarski_tarski_interp I), rho; repeat split.
+      + now exists l.
+      + easy.
+      + destruct I; apply Hdec.
+      + rewrite <- (full_interp_inverse_1 I) in H.
+        destruct (Hdec FSAT.P) as [fP HfP].
+        destruct (Hdec FSAT.less) as [fL HfL].
+        destruct (Hdec FSAT.equiv) as [fE HfE].
+        unshelve now eapply translate_form_correct in H.
+        intros ff phi rho'. apply Full.general_decider. 1: now exists l.
+        rewrite full_interp_inverse_1. intros ff' [] v ee; cbn;
+        apply DecidabilityFacts.decidable_iff'.
+        1: now exists fP. 1: now exists fL. now exists fE.
+    - exists D, (tarski_full_tarski_interp I), rho; repeat split.
+      + now exists l.
+      + easy.
+      + destruct I; apply Hdec.
+      + destruct (Hdec FSAT.P) as [fP HfP].
+        destruct (Hdec FSAT.less) as [fL HfL].
+        destruct (Hdec FSAT.equiv) as [fE HfE].
+        unshelve now eapply translate_form_correct.
+        intros ff phi rho'. apply Full.general_decider. 1: now exists l.
+        intros ff' [] v ee; cbn;
+        apply DecidabilityFacts.decidable_iff'; destruct I.
+        1: now exists fP. 1: now exists fL. now exists fE.
+  Qed.
 End Fragment.
